Cobb/underapproximation_type/data/predefined/templates.ml
@@ -13,6 +13,7 @@ let[@axiom] template_leq_1 (a : int) = a <= 1
 let[@axiom] template_emp (l : int list) = emp l
 let[@axiom] template_singleton (l : int list) = len l 1
 let[@axiom] template_sorted (l : int list) = sorted l
+let[@axiom] template_incr_one (l : int list) = incr_one l
 let[@axiom] template_leaf (l : int tree) = leaf l
 let[@axiom] template_rb_leaf (v : int rbtree) = rb_leaf v
 let[@axiom] template_no_red_red (v : int rbtree) = no_red_red v
