Cobb/underapproximation_type/data/validation/list_incr_one_max_sketch/prog.ml
@@ -1,0 +1,18 @@
+let rec incr_one_list_gen (s : int) (x : int) : int list =
+  if sizecheck s then []
+  else
+    let (y : int) = int_gen () in
+    if y == x + 1 then
+      let (size2 : int) = subs s in
+      let (l : int list) = incr_one_list_gen size2 y in
+      let (l2 : int list) = y :: l in
+      l2
+    else Exn
+
+let[@assert] incr_one_list_gen =
+  let s = ((0 <= v : [%v: int]) [@over]) in
+  let x = ((true : [%v: int]) [@over]) in
+  ((len v s && incr_one v
+    && (not (emp v)) #==> (fun ((u [@exists]) : int) -> hd v u && x <= u)
+    : [%v: int list])
+    [@under])
