Cobb/underapproximation_type/data/validation/twos_tree_min_sketch/prog.ml
@@ -1,11 +1,12 @@
 let rec twos_tree_gen (d : int) : int tree =
   if sizecheck d then Leaf
-  else if bool_gen () then Leaf 
-  else
+  else if bool_gen () then
     let (x : int) = two () in
     let (lt : int tree) = twos_tree_gen (subs d) in
     let (rt : int tree) = twos_tree_gen (subs d) in
     Node (x, lt, rt)
+  else Leaf 
+
 
 let[@assert] twos_tree_gen =
   let d = ((0 <= v : [%v: int]) [@over]) in
